theories/L/Functions/UnboundIteration.v
@@ -47,7 +47,7 @@ Section uiter.
   Lemma uiter_total_instanceTime {Z} `{registered Z} (f':  Z -> Y) (preprocess : Z -> X) preprocessT (fuel : Z -> nat)
     `{computableTime' preprocess preprocessT} :
     (forall x, loopSum (fuel x) f (preprocess x) = Some (f' x)) ->
-    computesTime (TyArr _ _) f' (λ x, uiter (extT preprocess x)) (fun z _ => (1 + fst (preprocessT z tt) + uiterTime (fuel z) (preprocess z),tt)).
+    computesTime (TyAll _ _) f' (λ x, uiter (extT preprocess x)) (fun z _ => (1 + fst (preprocessT z tt) + uiterTime (fuel z) (preprocess z),tt)).
   Proof.
     cbn [convert TH].
     intros total.
